src/linear/adt/Stack.dfy
@@ -4,7 +4,7 @@ include "../../../src/linear/interface/Stack.dfy"
 class Stack1 extends Stack {
   var list: List<int>;
 
-  function Depth(): nat
+  function ReprDepth(): nat
   {
     1
   }
